AVX2 encode12 spec equivalence proof

proof/correctness/avx2/Kyber_AVX2_cf.ec
@@ -1,5 +1,6 @@
-require import AllCore List Int IntDiv CoreMap Real Number LoopTransform.
-from Jasmin require import JWord.
+require import AllCore List Int IntDiv StdOrder CoreMap Real Number LoopTransform.
+import IntOrder.
+from Jasmin require import JModel.
 require import Array16 Array32 Array64 Array128 Array168 Array256 Array384.
 require import Jkem.
 require import Kyber.
@@ -52,6 +53,31 @@ module EncDec_AVX2 = {
     var r : ipoly;
     r <- witness;
     i <- 0;
+
+    while (i < 4) {
+      j <- 0;
+      while(j < 8){
+        r.[64*i+j*8+0] <- b2i a.[8*i+j].[0];
+        r.[64*i+j*8+1] <- b2i a.[8*i+j].[1];
+        r.[64*i+j*8+2] <- b2i a.[8*i+j].[2];
+        r.[64*i+j*8+3] <- b2i a.[8*i+j].[3];
+        r.[64*i+j*8+4] <- b2i a.[8*i+j].[4];
+        r.[64*i+j*8+5] <- b2i a.[8*i+j].[5];
+        r.[64*i+j*8+6] <- b2i a.[8*i+j].[6];
+        r.[64*i+j*8+7] <- b2i a.[8*i+j].[7];
+        j <- j + 1;
+      }
+      i<-i+1;
+    }
+
+    return r;
+  }
+
+  proc decode1_opt(a : W8.t Array32.t) : ipoly = {
+    var i,j;
+    var r : ipoly;
+    r <- witness;
+    i <- 0;
     while (i < 4) {
       j <- 0;
       while(j < 4) {
@@ -91,17 +117,37 @@ module EncDec_AVX2 = {
        k <- 0;
 
        while(k < 64) {
-         fi1 <- a.[128*i + k];
-         fi2 <- a.[128*i + k + 1];
+         fi1 <- a.[128*i + 2*k];
+         fi2 <- a.[128*i + 2*k + 1];
          r.[192*i+3*k] <- W8.of_int fi1;
          r.[192*i+3*k+1] <- W8.of_int ((fi2 %% 2^4) * 2^4 + fi1 %/ 2^8);
          r.[192*i+3*k+2] <- W8.of_int (fi2 %/ 2^4);
-         k <- k + 2;
+         k <- k + 1;
        }
 
        i <- i + 1;
      }
      return r;
+  }
+
+  proc encode12_opt(a : ipoly) : W8.t Array384.t = {
+    var fi1,fi2: int;
+    var i;
+    var r : W8.t Array384.t;
+
+    i <- 0;
+    while (i < 2) {
+
+      r <- fill (fun k => let fi1 = a.[128*i + 2 * (k %% 192 %/ 3)] in
+                          let fi2 = a.[128*i + 2 * (k %% 192 %/ 3) + 1] in
+                          if (k %% 3 = 0) then W8.of_int fi1
+                          else if (k %% 3 = 1) then W8.of_int ((fi2 %% 2^4) * 2^4 + fi1 %/ 2^8)
+                          else W8.of_int (fi2 %/ 2^4))
+                (192*i) 192 r;
+
+      i <- i + 1;
+    }
+    return r;
   }
 
    proc encode4(p : ipoly) : W8.t Array128.t = {
@@ -145,9 +191,6 @@ module EncDec_AVX2 = {
     }
     return ra;      
   }
-
-
-
 }.
 
 module Kyber_AVX2_cf = {
@@ -180,3 +223,93 @@ module Kyber_AVX2_cf = {
     return (r);
   }
 }.
+
+theory AVX2_cf.
+
+equiv eq_encode12:
+  EncDec_AVX2.encode12_opt ~ EncDec_AVX2.encode12: ={a} ==> ={res}.
+proof.
+  proc.
+  while (#pre /\ i{1} = i{2} /\ 0 <= i{1} <= 2 /\
+         (forall k, 0 <= k < 192 * i{1} => r{1}.[k] = r{2}.[k])).
+    unroll for {2} 2.
+    wp; skip; auto => />.
+    move => &1 &2 [#] i_lb i_ub r1_eq_r2 i_tub />.
+    split.
+      + move : i_lb i_tub => /#.
+      + rewrite (mulzDr 192 _ _) mulz1.
+        move => k k_lb k_ub.
+        rewrite filliE 1:/# //=.
+        rewrite k_ub //=.
+        case (k < 192 * i{2}) => k_tub.
+          + have -> //=: !(192 * i{2} <= k). move : k_tub => /#.
+            rewrite r1_eq_r2; first by rewrite k_lb k_tub.
+            do (rewrite Array384.set_neqiE 1:/#; first by move : k_tub k_lb => /#).
+            done.
+          + move : k_tub => -/lezNgt k_tlb.
+            rewrite k_tlb //=.
+            do (rewrite Array384.get_setE 1:/#).
+            have k_iota: k \in iota_ (192 * i{2}) 192; first by rewrite mem_iota k_ub k_tlb.
+            move : k_iota.
+            case (k %% 3 = 0) => k_m.
+              smt(@Array384 @Int @IntDiv @List).
+            case (k %% 3 = 1) => k_m_1.
+              smt(@Array384 @Int @IntDiv @List).
+            have k_m_2: k %% 3 = 2. move : k_m k_m_1 (modz_cmp k 3) => /#.
+              smt(@Array384 @Int @IntDiv @List).
+  wp; skip; auto => />.
+  move => &1 &2 *.
+  split.
+    smt(@Logic).
+    move => rL iR rR iR_tlb _ iR_lb iR_ub.
+    have -> //=: iR = 2. move : iR_tlb iR_ub => /#.
+    apply Array384.ext_eq.
+qed.
+
+equiv eq_decode4:
+  EncDec_AVX2.decode4 ~ EncDec.decode4: ={a} ==> ={res}.
+proof.
+  proc.
+  seq 2 2: (i{1} = 0 /\ ={a, r, i}) => //.
+  wp; skip; auto => />.
+  async while
+    [ (fun r => i < r), (i{1} + 1) ]
+    [ (fun r => i < 8 * r), (i{1} + 1) ]
+      (i{1} < 16 /\ i{2} < 16 * 8) (!(i{1} < 16))
+    :
+      (={r, a} /\ i{2} = 8 * i{1} /\ (0 <= i{2})) => //=.
+  + by move=> &1 &2 />; smt(@Int).
+  + by move=> &1 &2 />; smt(@Int).
+  + by move=> &1 &2 />; smt(@Int).
+  + by move=> &2 />; exfalso => &1; smt(@Int).
+  + by move=> &2 />; exfalso => &1; smt(@Int).
+  + move => v1 v2.
+    rcondt {1} 1; 1: by auto => /> /#.
+    rcondf {1} 4; 1: by auto; conseq (_: true); auto.
+    wp; while(={a, r}
+              /\ i{2} = 8 * i{1} + j{1}
+              /\ v1 = (i{1} + 1)
+              /\ 0 <= i{1} < 16
+              /\ 0 <= j{1} <= 8) => /=; last by auto; smt(@Int).
+    wp; skip => &1 &2 /= />.
+    move => i1_lb i1_tub j_lb j1_ub j1_tub si_ub si_tub />.
+    split.
+      split. smt(@Int).
+      smt(@Int).
+    split.
+      smt(@Int).
+      admit. (* FIXME *)
+    while true (16 - i) => //; auto => />.
+      unroll for 2.
+      wp. skip. trivial.
+    auto => /#.
+    while true (128 - i); last first.
+    wp; skip; auto => /#.
+    move => z; wp. auto => /#.
+  (* TODO *)
+  admit.
+qed.
+
+
+
+end AVX2_cf.
